coq/coq/syntax_ott.v
@@ -63,7 +63,7 @@ Definition ctx : Set := list ( atom * typ ).
 (** opening up abstractions *)
 Fixpoint open_texp_wrt_texp_rec (k:nat) (t_5:texp) (t__6:texp) {struct t__6}: texp :=
   match t__6 with
-  | (texp_var_b nat) =>
+  | (texp_var_b nat) => 
       match lt_eq_lt_dec nat k with
         | inleft (left _) => texp_var_b nat
         | inleft (right _) => t_5
@@ -74,7 +74,7 @@ Fixpoint open_texp_wrt_texp_rec (k:nat) (t_5:texp) (t__6:texp) {struct t__6}: te
   | (texp_abs t) => texp_abs (open_texp_wrt_texp_rec (S k) t_5 t)
   | (texp_fixpoint t) => texp_fixpoint (open_texp_wrt_texp_rec (S k) t_5 t)
   | (texp_app t1 t2) => texp_app (open_texp_wrt_texp_rec k t_5 t1) (open_texp_wrt_texp_rec k t_5 t2)
-  | texp_nil => texp_nil
+  | texp_nil => texp_nil 
   | (texp_cons l t1' t2) => texp_cons l (open_texp_wrt_texp_rec k t_5 t1') (open_texp_wrt_texp_rec k t_5 t2)
   | (texp_proj t1 l) => texp_proj (open_texp_wrt_texp_rec k t_5 t1) l
   | (texp_concat t1 t2) => texp_concat (open_texp_wrt_texp_rec k t_5 t1) (open_texp_wrt_texp_rec k t_5 t2)
@@ -82,9 +82,9 @@ end.
 
 Fixpoint open_exp_wrt_exp_rec (k:nat) (e_5:exp) (e__6:exp) {struct e__6}: exp :=
   match e__6 with
-  | exp_top => exp_top
+  | exp_top => exp_top 
   | (exp_base b) => exp_base b
-  | (exp_var_b nat) =>
+  | (exp_var_b nat) => 
       match lt_eq_lt_dec nat k with
         | inleft (left _) => exp_var_b nat
         | inleft (right _) => e_5
@@ -123,7 +123,7 @@ Inductive lc_texp : texp -> Prop :=    (* defn lc_texp *)
      (lc_texp t1) ->
      (lc_texp t2) ->
      (lc_texp (texp_app t1 t2))
- | lc_texp_nil :
+ | lc_texp_nil : 
      (lc_texp texp_nil)
  | lc_texp_cons : forall (l:label) (t1' t2:texp),
      (lc_texp t1') ->
@@ -139,7 +139,7 @@ Inductive lc_texp : texp -> Prop :=    (* defn lc_texp *)
 
 (* defns LC_exp *)
 Inductive lc_exp : exp -> Prop :=    (* defn lc_exp *)
- | lc_exp_top :
+ | lc_exp_top : 
      (lc_exp exp_top)
  | lc_exp_base : forall (b:lit),
      (lc_exp (exp_base b))
@@ -201,7 +201,7 @@ end.
 (** substitutions *)
 Fixpoint esubst_exp (e_5:exp) (x5:var) (e__6:exp) {struct e__6} : exp :=
   match e__6 with
-  | exp_top => exp_top
+  | exp_top => exp_top 
   | (exp_base b) => exp_base b
   | (exp_var_b nat) => exp_var_b nat
   | (exp_var_f x) => (if eq_var x x5 then e_5 else (exp_var_f x))
@@ -222,7 +222,7 @@ Fixpoint subst_texp (t_5:texp) (x5:var) (t__6:texp) {struct t__6} : texp :=
   | (texp_abs t) => texp_abs (subst_texp t_5 x5 t)
   | (texp_fixpoint t) => texp_fixpoint (subst_texp t_5 x5 t)
   | (texp_app t1 t2) => texp_app (subst_texp t_5 x5 t1) (subst_texp t_5 x5 t2)
-  | texp_nil => texp_nil
+  | texp_nil => texp_nil 
   | (texp_cons l t1' t2) => texp_cons l (subst_texp t_5 x5 t1') (subst_texp t_5 x5 t2)
   | (texp_proj t1 l) => texp_proj (subst_texp t_5 x5 t1) l
   | (texp_concat t1 t2) => texp_concat (subst_texp t_5 x5 t1) (subst_texp t_5 x5 t2)
@@ -257,7 +257,7 @@ Definition list_string_2_string (l : LS) : string :=
   fold_left append l "".
 
 Coercion list_string_2_string : LS >-> string.
-Locate merge.
+
 Fixpoint stype2string (A: typ) : LS :=
   if (check_toplike A) then nil
   else
@@ -269,7 +269,7 @@ Fixpoint stype2string (A: typ) : LS :=
     | typ_rcd l A' => ["{" ++  l ++ "=>" ++ (stype2string A') ++ "}"]
     | typ_and A1 A2 => nodup string_dec (merge (stype2string A1) (stype2string A2))
     end.
-
+    
 Notation "|| A ||" := (stype2string A) (at level 50, A at next level). (* 1 is too high *)
 
 Fixpoint ttyp_concat_simpl (A: ttyp) (B: ttyp) :=
@@ -313,7 +313,7 @@ Fixpoint Tlookup (i:string) (T:ttyp) : option ttyp :=
 
 (* defns TopLikeType *)
 Inductive toplike : typ -> Prop :=    (* defn toplike *)
- | TL_top :
+ | TL_top : 
      toplike typ_top
  | TL_and : forall (A B:typ),
      toplike A ->
@@ -363,19 +363,19 @@ Inductive eqIndTyp : typ -> typ -> Prop :=    (* defn eqIndTyp *)
 (* defns SplitType *)
 Inductive spl : typ -> typ -> typ -> Prop :=    (* defn spl *)
  | Sp_and : forall (A B:typ),
-     spl  (typ_and A B)   A   B
+     spl  (typ_and A B)   A   B 
  | Sp_arrow : forall (A B B1 B2:typ),
      spl B B1 B2 ->
-     spl  (typ_arrow A B)   (typ_arrow A B1)   (typ_arrow A B2)
+     spl  (typ_arrow A B)   (typ_arrow A B1)   (typ_arrow A B2) 
  | Sp_rcd : forall (l:label) (B B1 B2:typ),
      spl B B1 B2 ->
      spl (typ_rcd l B) (typ_rcd l B1) (typ_rcd l B2).
 
 (* defns OrdinaryType *)
 Inductive ord : typ -> Prop :=    (* defn ord *)
- | O_top :
+ | O_top : 
      ord typ_top
- | O_int :
+ | O_int : 
      ord typ_base
  | O_arrow : forall (A B:typ),
      ord B ->
@@ -428,7 +428,7 @@ Inductive comerge : texp -> typ -> typ -> texp -> typ -> texp -> Prop :=    (* d
      comerge t1 A (typ_and A B) t2 B (texp_concat t1 t2)
  | M_Arrow : forall (L:vars) (t1:texp) (A B1 B:typ) (t2:texp) (B2:typ) (t:texp),
       ( forall x , x \notin  L  -> comerge (texp_app   (texp_proj  t1  (stype2string  (typ_arrow A B1) ))   (texp_var_f x)) B1 B (texp_app   (texp_proj  t2  (stype2string  (typ_arrow A B2) ))   (texp_var_f x)) B2  ( open_texp_wrt_texp t (texp_var_f x) )  )  ->
-     comerge t1 (typ_arrow A B1) (typ_arrow A B) t2 (typ_arrow A B2)  (texp_cons (stype2string  (typ_arrow A B) )  (texp_abs t)  texp_nil)
+     comerge t1 (typ_arrow A B1) (typ_arrow A B) t2 (typ_arrow A B2)  (texp_cons (stype2string  (typ_arrow A B) )  (texp_abs t)  texp_nil) 
  | M_Rcd : forall (t1:texp) (l:label) (A1 A:typ) (t2:texp) (A2:typ) (t:texp),
      comerge  (texp_proj  t1  (stype2string  (typ_rcd l A1) ))  A1 A  (texp_proj  t2  (stype2string  (typ_rcd l A2) ))  A2 t ->
      comerge t1 (typ_rcd l A1) (typ_rcd l A) t2 (typ_rcd l A2)  (texp_cons (stype2string  (typ_rcd l A) )  t  texp_nil) .
@@ -444,20 +444,20 @@ Inductive cosub : texp -> typ -> typ -> texp -> Prop :=    (* defn cosub *)
      lc_texp t ->
      ord B ->
       not ( toplike B )  ->
-     cosub t typ_bot B  (texp_cons (stype2string  B )  (texp_fixpoint (texp_var_b 0))  texp_nil)
+     cosub t typ_bot B  (texp_cons (stype2string  B )  (texp_fixpoint (texp_var_b 0))  texp_nil) 
  | S_Base : forall (t:texp),
      lc_texp t ->
-     cosub t typ_base typ_base  (texp_cons (stype2string  typ_base )   (texp_proj  t  (stype2string  typ_base ))   texp_nil)
+     cosub t typ_base typ_base  (texp_cons (stype2string  typ_base )   (texp_proj  t  (stype2string  typ_base ))   texp_nil) 
  | S_Arrow : forall (L:vars) (t:texp) (A1 A2 B1 B2:typ) (t2 t1:texp),
      ord B2 ->
       not ( toplike B2 )  ->
       ( forall x , x \notin  L  ->  ( cosub (texp_var_f x) B1 A1 t1  /\  cosub (texp_app   (texp_proj  t  (stype2string  (typ_arrow A1 A2) ))   t1) A2 B2  ( open_texp_wrt_texp t2 (texp_var_f x) )  )  )  ->
-     cosub t (typ_arrow A1 A2) (typ_arrow B1 B2)  (texp_cons (stype2string  (typ_arrow B1 B2) )  (texp_abs t2)  texp_nil)
+     cosub t (typ_arrow A1 A2) (typ_arrow B1 B2)  (texp_cons (stype2string  (typ_arrow B1 B2) )  (texp_abs t2)  texp_nil) 
  | S_Rcd : forall (t:texp) (l:label) (A B:typ) (t2:texp),
      ord B ->
       not ( toplike B )  ->
      cosub  (texp_proj  t  (stype2string  (typ_rcd l A) ))  A B t2 ->
-     cosub t (typ_rcd l A) (typ_rcd l B)  (texp_cons (stype2string  (typ_rcd l B) )  t2  texp_nil)
+     cosub t (typ_rcd l A) (typ_rcd l B)  (texp_cons (stype2string  (typ_rcd l B) )  t2  texp_nil) 
  | S_AndL : forall (t:texp) (A B C:typ) (t':texp),
      ord C ->
      cosub t A C t' ->
@@ -475,14 +475,18 @@ Inductive cosub : texp -> typ -> typ -> texp -> Prop :=    (* defn cosub *)
 
 (* defns Subtyping *)
 Inductive sub : typ -> typ -> Prop :=    (* defn sub *)
- | S_z :
+ | S_z : 
      sub typ_base typ_base
  | S_top : forall (A B:typ),
      toplike B ->
      sub A B
+ | S_bot : 
+     sub typ_bot typ_bot
  | S_arr : forall (A1 A2 B1 B2:typ),
      sub B1 A1 ->
+     sub A1 B1 ->
      sub A2 B2 ->
+     sub B2 A2 ->
      sub (typ_arrow A1 A2) (typ_arrow B1 B2)
  | S_andl1 : forall (A1 A2 A3:typ),
      sub A1 A3 ->
@@ -545,7 +549,7 @@ Inductive elaboration : ctx -> exp -> dirflag -> typ -> texp -> Prop :=    (* de
      elaboration G (exp_rcd l e) Inf (typ_rcd l A) texp_nil
  | Ela_Base : forall (G:ctx) (b:lit),
       uniq  G  ->
-     elaboration G (exp_base b) Inf typ_base  (texp_cons (stype2string  typ_base )  (texp_base b)  texp_nil)
+     elaboration G (exp_base b) Inf typ_base  (texp_cons (stype2string  typ_base )  (texp_base b)  texp_nil) 
  | Ela_Var : forall (G:ctx) (x:var) (A:typ),
       uniq  G  ->
       binds  x A G  ->
@@ -555,7 +559,7 @@ Inductive elaboration : ctx -> exp -> dirflag -> typ -> texp -> Prop :=    (* de
      elaboration G (exp_fixpoint A e) Inf A (texp_fixpoint t)
  | Ela_Abs : forall (L:vars) (G:ctx) (A:typ) (e:exp) (B:typ) (t:texp),
       ( forall x , x \notin  L  -> elaboration  (cons ( x , A )  G )   ( open_exp_wrt_exp e (exp_var_f x) )  Chk B  ( open_texp_wrt_texp t (texp_var_f x) )  )  ->
-     elaboration G (exp_abs A e B) Inf (typ_arrow A B)  (texp_cons (stype2string  (typ_arrow A B) )  (texp_abs t)  texp_nil)
+     elaboration G (exp_abs A e B) Inf (typ_arrow A B)  (texp_cons (stype2string  (typ_arrow A B) )  (texp_abs t)  texp_nil) 
  | Ela_App : forall (G:ctx) (e1 e2:exp) (C:typ) (t3:texp) (A:typ) (t1:texp) (B':typ) (t2:texp),
      elaboration G e1 Inf A t1 ->
      elaboration G e2 Inf B' t2 ->
@@ -563,7 +567,7 @@ Inductive elaboration : ctx -> exp -> dirflag -> typ -> texp -> Prop :=    (* de
      elaboration G (exp_app e1 e2) Inf C t3
  | Ela_Rcd : forall (G:ctx) (l:label) (e:exp) (A:typ) (t:texp),
      elaboration G e Inf A t ->
-     elaboration G (exp_rcd l e) Inf (typ_rcd l A)  (texp_cons (stype2string  (typ_rcd l A) )  t  texp_nil)
+     elaboration G (exp_rcd l e) Inf (typ_rcd l A)  (texp_cons (stype2string  (typ_rcd l A) )  t  texp_nil) 
  | Ela_Proj : forall (G:ctx) (e:exp) (l:label) (B:typ) (t2:texp) (A:typ) (t1:texp),
      elaboration G e Inf A t1 ->
      proj t1 A l t2 B ->
@@ -583,7 +587,7 @@ Inductive elaboration : ctx -> exp -> dirflag -> typ -> texp -> Prop :=    (* de
 
 (* defns Values *)
 Inductive value : texp -> Prop :=    (* defn value *)
- | value_unit :
+ | value_unit : 
      value texp_nil
  | value_lit : forall (b:lit),
      value (texp_base b)
@@ -639,14 +643,14 @@ Inductive target_step : texp -> texp -> Prop :=    (* defn target_step *)
  | TS_AppAbs : forall (t tv:texp),
      lc_texp (texp_abs t) ->
      lc_texp tv ->
-     target_step (texp_app  (texp_abs t)  tv)  (open_texp_wrt_texp  t tv )
+     target_step (texp_app  (texp_abs t)  tv)  (open_texp_wrt_texp  t tv ) 
  | TS_Fixpoint : forall (t:texp),
      lc_texp (texp_fixpoint t) ->
      target_step (texp_fixpoint t)  (open_texp_wrt_texp  t (texp_fixpoint t) ) .
 
 (* defns RecordTypes *)
 Inductive rec_typ : ttyp -> Prop :=    (* defn rec_typ *)
- | RT_Nil :
+ | RT_Nil : 
      rec_typ ttyp_top
  | RT_Rcd : forall (l:label) (At Bt:ttyp),
      rec_typ Bt ->
@@ -654,11 +658,11 @@ Inductive rec_typ : ttyp -> Prop :=    (* defn rec_typ *)
 
 (* defns TargetEqIndexType *)
 Inductive eqIndTypTarget : ttyp -> ttyp -> Prop :=    (* defn eqIndTypTarget *)
- | TEI_top :
+ | TEI_top : 
      eqIndTypTarget ttyp_top ttyp_top
- | TEI_bot :
+ | TEI_bot : 
      eqIndTypTarget ttyp_bot ttyp_bot
- | TEI_base :
+ | TEI_base : 
      eqIndTypTarget ttyp_base ttyp_base
  | TEI_arrow : forall (At1 Bt1 At2 Bt2:ttyp),
      eqIndTypTarget At1 At2 ->
@@ -700,11 +704,11 @@ Inductive contained_by_rec_typ : ttyp -> label -> ttyp -> Prop :=    (* defn con
 
 (* defns WelformedTypes *)
 Inductive wf_typ : ttyp -> Prop :=    (* defn wf_typ *)
- | WF_Nil :
+ | WF_Nil : 
      wf_typ ttyp_top
- | WF_Bot :
+ | WF_Bot : 
      wf_typ ttyp_bot
- | WF_Base :
+ | WF_Base : 
      wf_typ ttyp_base
  | WF_Rcd : forall (l:label) (At Bt At':ttyp),
      wf_typ At ->
@@ -719,8 +723,8 @@ Inductive wf_typ : ttyp -> Prop :=    (* defn wf_typ *)
 
 (* defns WelformedCtx *)
 Inductive wf_ctx : tctx -> Prop :=    (* defn wf_ctx *)
- | WFC_Nil :
-     wf_ctx  nil
+ | WFC_Nil : 
+     wf_ctx  nil 
  | WFC_Cons : forall (Gt:tctx) (x:var) (At:ttyp),
      wf_typ At ->
      wf_ctx Gt ->
@@ -778,7 +782,7 @@ Inductive target_typing : tctx -> texp -> ttyp -> Prop :=    (* defn target_typi
       (   (  Tlookup  l   Bt  = Some  At'   /\  eqIndTypTarget At' At )    \/   Tlookup  l   Bt  = None  )  ->
      target_typing Gt t1 At ->
      target_typing Gt t2 Bt ->
-     target_typing Gt  (texp_cons l t1 t2)   (ttyp_rcd l At Bt)
+     target_typing Gt  (texp_cons l t1 t2)   (ttyp_rcd l At Bt) 
  | TTyping_RcdProj : forall (Gt:tctx) (t:texp) (l:label) (Bt At:ttyp),
      target_typing Gt t At ->
       Tlookup  l   At  = Some  Bt  ->
@@ -794,3 +798,5 @@ Inductive target_typing : tctx -> texp -> ttyp -> Prop :=    (* defn target_typi
 
 (** infrastructure *)
 Hint Constructors toplike eqIndTyp spl ord disjoint comerge cosub sub proj distapp elaboration value target_step rec_typ eqIndTypTarget concat_typ contained_by_rec_typ wf_typ wf_ctx SubtypeTarget target_typing lc_texp lc_exp : core.
+
+
